src/test/test1_AX_OR_V.v
@@ -1,0 +1,113 @@
+Require Import MC_CTL2.
+Require Import List. Import ListNotations.
+Require Import Lia.
+
+Ltac solve_fV init_ := (*solve satisfies model (fV ?) (?st) problem *)
+  repeat split;
+  let pre := fresh "pre" in
+  intro pre; 
+  rewrite init_ in pre; 
+  (discriminate)+auto
+.
+
+Ltac solve_fOr init_ tac1 tac2  := 
+(left; progress tac1 init_;progress auto) + (right; progress tac2 init_; progress auto) 
+.
+
+Ltac solve_fAX init_l tac1 := 
+  let next_state := fresh "next_state" in 
+  intro next_state;
+  let trans_to_new_state := fresh "trans_to_new_state" 
+  in 
+  intro trans_to_new_state;
+  compute in trans_to_new_state;
+  repeat (
+    let a := fresh "a" in
+    let b := fresh "b" in
+    destruct trans_to_new_state as (a&b);
+    ((apply a in init_l)+(apply b in init_l));
+    (
+      lazymatch type of init_l with 
+      | _ \/ _ => repeat( destruct init_l as [init_l|init_l])
+      | _ => idtac
+      end
+    ));
+    tac1 init_l.
+
+Ltac solve_fAnd tac1 tac2 init_ :=
+split; [> tac1 init_ | tac2 init_].
+
+
+Fixpoint make_disjucntion_for_state_to{A} (s2: A)(states_in: list A) := 
+match states_in with
+| head :: nil => s2 = head
+| head :: tail => s2 = head \/ (make_disjucntion_for_state_to s2 tail)
+| nil => False
+end
+.
+
+Fixpoint make_prop{A B} (s1:A )( s2:B) (list_connections: list (A * (list B))):Prop := 
+match list_connections with 
+| (b1,b2)::nil => (s1 = b1 -> (make_disjucntion_for_state_to s2 b2))
+| (b1,b2)::tail => (s1 = b1 -> (make_disjucntion_for_state_to s2 b2)) /\ (make_prop s1 s2 tail)
+| nil => False  
+end 
+.
+Definition to_Prop{A B}(list_connections: list (B * (list A))): B -> A -> Prop :=
+(fun s1 s2 => make_prop s1 s2 list_connections).
+
+
+Inductive   square' : Set :=  one_square' | two_square' | three_square' | four_square' .
+Definition  trans_square' := to_Prop [
+  (one_square', [two_square'; three_square';four_square']);
+  (two_square', [two_square']);
+  (three_square', [three_square']);
+  (four_square', [four_square'])
+].
+
+
+Definition  label_square' := to_Prop [
+(one_square', [0]);
+(two_square', [1]); 
+(three_square', [1]); 
+(four_square', [2])].
+
+
+
+Definition  serial_square': forall w:square', exists (v:square'), trans_square' w v.
+intros.
+case w.
+eexists two_square';repeat split; intro;try discriminate;left;auto.
+eexists two_square';repeat split; intro;try discriminate; auto.
+eexists three_square';repeat split; intro;try discriminate; auto.
+eexists four_square';repeat split; intro;try discriminate; auto.
+Defined.
+
+Definition init_square' := fun st => st = one_square'.
+Definition model_square': sts :=  {| 
+  state   := square'; 
+  trans   := trans_square'; 
+  init    := init_square'; 
+  label   := fun a b => label_square' b a; 
+  serial  := serial_square' 
+|}.
+
+Theorem F1: 
+forall st: state model_square', 
+(init model_square') st -> 
+satisfies (model_square') (fAX (fOr (fV 1) (fOr (fV 1) (fV 2)))) st.
+Proof.
+intro st.
+intro init_l.
+let sol := 
+    let sol_or := 
+    (fun init_ => solve_fOr init_ solve_fV solve_fV)
+    in
+    (fun init_ => solve_fOr init_ solve_fV sol_or)
+in
+solve_fAX init_l sol.
+
+
+
+
+
