src/test/test2_AU.v
@@ -1,0 +1,453 @@
+Require Import MC_CTL2.
+Require Import List. Import ListNotations.
+Require Import Lia.
+
+Ltac solve_fV init_ := (*solve satisfies model (fV ?) (?st) problem *)
+  repeat split;
+  let pre := fresh "pre" in
+  intro pre; 
+  rewrite init_ in pre; 
+  (discriminate)+auto
+.
+
+Ltac solve_fOr init_ tac1 tac2  := 
+(left; progress tac1 init_;progress auto) + (right; progress tac2 init_; progress auto) 
+.
+
+Ltac solve_fAX init_l tac1 := 
+  let next_state := fresh "next_state" in 
+  intro next_state;
+  let trans_to_new_state := fresh "trans_to_new_state" 
+  in 
+  intro trans_to_new_state;
+  compute in trans_to_new_state;
+  repeat (
+    let a := fresh "a" in
+    let b := fresh "b" in
+    destruct trans_to_new_state as (a&b);
+    ((apply a in init_l)+(apply b in init_l));
+    (
+      lazymatch type of init_l with 
+      | _ \/ _ => repeat( destruct init_l as [init_l|init_l])
+      | _ => idtac
+      end
+    ));
+    tac1 init_l.
+
+Ltac solve_fAnd tac1 tac2 init_ :=
+split; [> tac1 init_ | tac2 init_].
+
+
+Fixpoint make_disjucntion_for_state_to{A} (s2: A)(states_in: list A) := 
+match states_in with
+| head :: nil => s2 = head
+| head :: tail => s2 = head \/ (make_disjucntion_for_state_to s2 tail)
+| nil => False
+end
+.
+
+Fixpoint make_prop{A B} (s1:A )( s2:B) (list_connections: list (A * (list B))):Prop := 
+match list_connections with 
+| (b1,b2)::nil => (s1 = b1 -> (make_disjucntion_for_state_to s2 b2))
+| (b1,b2)::tail => (s1 = b1 -> (make_disjucntion_for_state_to s2 b2)) /\ (make_prop s1 s2 tail)
+| nil => False  
+end 
+.
+Definition to_Prop{A B}(list_connections: list (B * (list A))): B -> A -> Prop :=
+(fun s1 s2 => make_prop s1 s2 list_connections).
+
+
+
+Theorem usefull4: forall m n, S m = n -> m = n - 1.
+lia.
+Defined.
+Definition usefull: forall m n:nat, S m <= n -> S m = n \/ S m <= n - 1.
+lia.
+Defined. 
+
+Definition usefull2: forall m n:nat, S m = S n -> m = n .
+lia.
+Defined.
+Definition usefull3: forall m n:nat, m <= n -> m - 1 <= n - 1.
+lia.
+Defined.
+
+
+
+Ltac solve_AU n max_of_state init_l solve_subformula1 solve_subformula2 := 
+let solve_AU max_of_state :=
+    let path_pi := fresh "path_pi" in
+    intro path_pi;
+    let is_path_pi := fresh "is_path_pi" in
+    intro is_path_pi;
+    let first_state:= fresh "first_state" in
+    intro first_state;
+    compute;
+    let (*rec*) sol_AU n :=
+    (* tryif (let h:= fresh "h" in assert(h: n <= max_of_state); [progress auto | auto])
+    then *)
+    (
+        eexists n (*n*); 
+        [
+            auto;
+            let m := fresh "m" in
+            let le_m := fresh "le_m" in
+            intro m;
+            intro le_m;
+            (
+            let rec solve_rec le_m := 
+                apply usefull in le_m; (*compute in le_m;*)
+                destruct le_m as [ le_m | le_m];
+                [>
+                (apply usefull2 in le_m) + lia (* for cases S m = 0*);
+                rewrite init_l in first_state;
+                try (rewrite <- le_m in first_state;
+                solve_subformula1 first_state);
+                let rec loop_to_needed_m i m :=
+                    tryif (let h:= fresh "h" in assert(h: i < m); [progress auto | auto])
+                    then 
+                        let is_path_pi_i := fresh "is_path_pi_i" in
+                        pose proof (is_path_pi i) as is_path_pi_i;
+                        compute in is_path_pi_i;
+                        repeat (
+                            let a := fresh "a" in
+                            let b := fresh "b" in
+                            destruct is_path_pi_i as (a&b);
+                            ((apply a in first_state)+(apply b in first_state));
+                            (
+                            lazymatch type of first_state with 
+                            | _ \/ _ => (repeat destruct first_state as [first_state|first_state])
+                            | _ => idtac
+                            end
+                            );
+                            loop_to_needed_m (i + 1) m)
+                    else 
+                        idtac
+                in
+                lazymatch type of le_m with 
+                | _ = ?k => loop_to_needed_m 0 k
+                | _ => idtac
+                end
+                ;
+                rewrite <- le_m in first_state;
+                solve_subformula1 first_state
+                
+                |
+                (compute in le_m;
+                lia) +  
+                (solve_rec le_m) + auto
+                ]
+            in
+            (solve_rec le_m)
+            )
+            
+        |
+        auto;
+        rewrite init_l in first_state;
+        let rec loop_to_needed_m i m :=
+            tryif (let h:= fresh "h" in assert(h: i < m); [progress auto | auto])
+            then 
+                let is_path_pi_i := fresh "is_path_pi_i" in
+                pose proof (is_path_pi i) as is_path_pi_i;
+                compute in is_path_pi_i;
+                repeat (
+                    let a := fresh "a" in
+                    let b := fresh "b" in
+                    destruct is_path_pi_i as (a&b);
+                    ((apply a in first_state)+(apply b in first_state));
+                    (repeat (
+                    lazymatch type of first_state with 
+                    | _ \/ _ => (destruct first_state as [first_state|first_state])
+                    | _ => idtac
+                    end
+                    ));
+                    loop_to_needed_m (i + 1) m)
+            else 
+                idtac
+        in
+        loop_to_needed_m 0 n;
+        solve_subformula2 first_state
+        ]
+    )
+    (* +
+    sol_AU (n + 1)
+    else 
+    fail "solve_AU: with" n*)
+    in 
+    sol_AU n
+in
+solve_AU max_of_state.
+
+
+Inductive square : Set :=  
+| one_square 
+| two_square
+| three_square
+| four_square 
+| five_square
+| six_square .
+Definition  trans_square := to_Prop [
+(one_square, [two_square; five_square]);
+(two_square, [three_square; five_square]);
+(three_square, [four_square] );
+(four_square, [four_square]);
+(five_square, [three_square; six_square]);
+(six_square , [six_square])
+].
+
+
+Definition  label_square := to_Prop [
+(one_square, [0]);
+(two_square, [0]);
+(three_square, [0]);
+(four_square, [1]);
+(five_square, [0]);
+(six_square ,[1])
+].
+
+Definition  serial_square: forall w:square, exists (v:square), trans_square w v.
+intros.
+case w.
+eexists two_square;repeat split; intro;try discriminate;left;auto.
+eexists three_square;repeat split; intro;try discriminate;left;auto.
+eexists four_square;repeat split; intro;try discriminate;left;auto.
+eexists four_square;repeat split; intro;try discriminate;left;auto.
+eexists three_square;repeat split; intro;try discriminate;left;auto.
+eexists six_square;repeat split; intro;try discriminate;left;auto.
+Defined.
+
+Definition init_square := fun st => st = one_square.
+Definition model_square: sts :=  {| 
+  state   := square; 
+  trans   := trans_square; 
+  init    := init_square; 
+  label   := fun a b => label_square b a; 
+  serial  := serial_square 
+|}.
+
+Ltac unsplit H1 H2 H12 :=
+lazymatch type of H1 with
+| ?t1 => 
+  lazymatch type of H2 with 
+  | ?t2 => 
+    assert (H12: t1 /\ t2)
+  end
+end  
+.
+
+
+Ltac next_state_gen i is_path_pi first_state :=
+  let is_path_pi_i := fresh "is_path_pi_i" in
+  pose proof (is_path_pi i) as is_path_pi_i;
+  compute in is_path_pi_i;
+  let a := fresh "a" in
+  let b := fresh "b" in
+  destruct is_path_pi_i as (a&b);
+  ((compute in a; apply a in first_state)+(apply b in first_state));
+  (repeat (
+  lazymatch type of first_state with 
+  | _ \/ _ => (destruct first_state as [first_state|first_state])
+  | _ => idtac
+  end
+  )).
+
+
+
+Theorem F1: 
+forall st: state model_square, 
+(init model_square) st -> 
+satisfies (model_square) (fAU (fV 0) (fV 1)) st.
+Proof.
+intro st.
+intro init_l.
+intro.
+intro is_path_pi.
+intro first_state.
+(* compute. *)
+rewrite init_l in first_state.
+(* 
+tac = n :=
+tryif i=0
+then 
+
+
+*)
+(* let prev_H := first_state in
+let H := fresh "H" in
+let new := fresh "first_state" in
+assert(new:=prev_H);
+next_state_gen 0 is_path_pi new;
+let new_acc := fresh "new_acc" in
+unsplit  new prev_H new_acc; auto.
+
+let prev_H := new_acc in
+let H := fresh "H" in
+let new := fresh "first_state" in
+next_state_gen (0+1) is_path_pi new.
+assert(new:=prev_H).
+let new_acc := fresh "new_acc" in
+unsplit  new prev_H new_acc; auto. *)
+
+let rec loop i n last_stop prev_acc write_here :=
+(
+  tryif (assert (i=n); [progress lia | auto])
+  then 
+    assert(write_here:=prev_acc)
+  else
+    let new := fresh "first_state" in
+    assert(new:=last_stop)
+    ;
+    next_state_gen i is_path_pi new;
+    let new_acc := fresh "new_acc" in
+    let H := fresh "H" in
+    unsplit new prev_acc H; auto
+    ;loop (i+1) n new H write_here
+)
+in
+let acc := fresh "seq" in
+loop 0 6 first_state first_state acc.
+{
+  
+  let proof_ex_sat i seq := 
+  eexists i; compute; [
+  
+  let m := fresh "m" in intro m; let lt_m := fresh "lt_m" in  intro lt_m;
+  let a := fresh "a" in
+  let b := fresh "b" in
+  destruct seq as (a&b);
+  let rec loop i sequence lt_m := 
+    lazymatch type of sequence with 
+    | _ /\ _ =>
+        let head := fresh "head" in
+        let tail := fresh "tail" in
+        destruct sequence as (head & tail);
+        apply usefull in lt_m;destruct lt_m as [lt_m| lt_m]; compute in lt_m; [
+          apply usefull4 in lt_m; compute in lt_m ;rewrite lt_m;
+          (* tac1 *) solve_fV head
+          |
+          (loop (i-1) tail lt_m)
+        ] 
+    | _ => 
+          apply usefull in lt_m;destruct lt_m as [lt_m| lt_m]; compute in lt_m; [
+          apply usefull4 in lt_m; compute in lt_m ;rewrite lt_m;
+          (* tac1 *) solve_fV sequence
+          |
+          (lia)
+        ]
+    end
+    in
+    loop i b lt_m
+    | 
+    let a := fresh "a" in
+    let b := fresh "b" in
+    destruct seq as (a&b);
+    solve_fV a
+  ] in
+  let rec big_loop i seq :=
+    lazymatch type of seq with 
+    | _ /\ _ =>
+      let a :=fresh "a" in
+      let b :=fresh "b" in
+      destruct seq as (a&b);
+      
+      (solve [proof_ex_sat (i-1) b]) +
+      (big_loop (i-1) b)
+      
+    | _ => idtac
+    end
+  in
+  big_loop 6 seq.
+
+}
+{
+  eexists 4.
+  let m := fresh "m" in intro m; let lt_m := fresh "lt_m" in  intro lt_m.
+
+  apply usefull in lt_m;destruct lt_m as [lt_m| lt_m]; compute in lt_m.
+  apply usefull4 in lt_m; compute in lt_m ;rewrite lt_m.
+  (* tac1 *) solve_fV first_state2.
+
+  apply usefull in lt_m;destruct lt_m as [lt_m| lt_m]; compute in lt_m.
+  apply usefull4 in lt_m; compute in lt_m ;rewrite lt_m.
+  (* tac1 *) solve_fV first_state1.
+
+  apply usefull in lt_m;destruct lt_m as [lt_m| lt_m]; compute in lt_m.
+  apply usefull4 in lt_m; compute in lt_m ;rewrite lt_m.
+  (* tac1 *) solve_fV first_state0.
+
+  apply usefull in lt_m;destruct lt_m as [lt_m| lt_m]; compute in lt_m.
+  apply usefull4 in lt_m; compute in lt_m ;rewrite lt_m.
+  (* tac1 *) solve_fV first_state.
+
+  lia.
+
+  (*tac2 *)solve_fV first_state3.
+}
+{
+  eexists 3.
+  let m := fresh "m" in intro m; let lt_m := fresh "lt_m" in  intro lt_m.
+
+  apply usefull in lt_m;destruct lt_m as [lt_m| lt_m]; compute in lt_m.
+  apply usefull4 in lt_m; compute in lt_m ;rewrite lt_m.
+  (* tac1 *) solve_fV first_state1.
+
+  apply usefull in lt_m;destruct lt_m as [lt_m| lt_m]; compute in lt_m.
+  apply usefull4 in lt_m; compute in lt_m ;rewrite lt_m.
+  solve_fV first_state0.
+
+  apply usefull in lt_m;destruct lt_m as [lt_m| lt_m]; compute in lt_m.
+  apply usefull4 in lt_m; compute in lt_m ;rewrite lt_m.
+  solve_fV first_state.
+
+  lia.
+
+  (*tac2 *)solve_fV first_state2.
+}
+{
+  eexists 3.
+  let m := fresh "m" in intro m; let lt_m := fresh "lt_m" in  intro lt_m.
+  apply usefull in lt_m;destruct lt_m as [lt_m| lt_m]; compute in lt_m.
+  apply usefull4 in lt_m; compute in lt_m ;rewrite lt_m.
+  (* tac1 *) solve_fV first_state1.
+
+  apply usefull in lt_m;destruct lt_m as [lt_m| lt_m]; compute in lt_m.
+  apply usefull4 in lt_m; compute in lt_m ;rewrite lt_m.
+  solve_fV first_state0.
+
+  apply usefull in lt_m;destruct lt_m as [lt_m| lt_m]; compute in lt_m.
+  apply usefull4 in lt_m; compute in lt_m ;rewrite lt_m.
+  solve_fV first_state.
+
+  lia.
+
+  (*tac2 *)solve_fV first_state2.
+
+}
+{
+  eexists 2.
+  let m := fresh "m" in intro m; let lt_m := fresh "lt_m" in  intro lt_m.
+
+  apply usefull in lt_m;destruct lt_m as [lt_m| lt_m]; compute in lt_m.
+  apply usefull4 in lt_m; compute in lt_m ;rewrite lt_m.
+  solve_fV first_state0.
+
+  apply usefull in lt_m;destruct lt_m as [lt_m| lt_m]; compute in lt_m.
+  apply usefull4 in lt_m; compute in lt_m ;rewrite lt_m.
+  solve_fV first_state.
+
+  lia.
+
+  (*tac2 *)solve_fV first_state1.
+}
+Defined.
+
+
+
+
+
+
+
+
+
+
+
